delimited continuations, unary model

theories/examples/delim_lang/adeq.v
@@ -5,6 +5,8 @@ From iris.algebra Require Import list.
 From iris.proofmode Require Import classes tactics.
 From iris.base_logic Require Import algebra.
 
+(* TODO: typing rules, if, compat for contexts, binary relation *)
+
 Require Import Binding.Lib Binding.Set Binding.Env.
 
 Open Scope syn.
@@ -16,88 +18,88 @@ Inductive ty :=
 
 Declare Scope types.
 
-Notation "τ '∕' α '→' σ '∕' β" := (Tarr τ α σ β) (at level 60) : types.
-Notation "'Cont' τ σ" := (Tcont τ σ) (at level 60) : types.
+(* Notation "τ '∕' α '→' σ '∕' β" := (Tarr τ α σ β) (at level 60) : types. *)
+(* Notation "'Cont' τ σ" := (Tcont τ σ) (at level 60) : types. *)
 
-Reserved Notation "Γ ';' α '⊢ₑ' e ':' τ ';' β"
-  (at level 90, e at next level, τ at level 20, no associativity).
+(* Reserved Notation "Γ ';' α '⊢ₑ' e ':' τ ';' β" *)
+(*   (at level 90, e at next level, τ at level 20, no associativity). *)
 
-Reserved Notation "Γ ';' α '⊢ᵥ' e ':' τ ';' β"
-  (at level 90, e at next level, τ at level 20, no associativity).
+(* Reserved Notation "Γ ';' α '⊢ᵥ' e ':' τ ';' β" *)
+(*   (at level 90, e at next level, τ at level 20, no associativity). *)
 
-Reserved Notation "Γ ';' α '⊢ᵪ' e ':' τ ';' β"
-  (at level 90, e at next level, τ at level 20, no associativity).
+(* Reserved Notation "Γ ';' α '⊢ᵪ' e ':' τ ';' β" *)
+(*   (at level 90, e at next level, τ at level 20, no associativity). *)
 
 (* TODO: pure stuff has ∀ σ deeper inside *)
-Inductive typed_expr {S : Set} (Γ : S -> ty) : ty -> expr S -> ty -> ty -> Prop :=
-| typed_Val v α τ β :
-  (Γ; α ⊢ᵥ v : τ; β) →
-  (Γ; α ⊢ₑ v : τ; β)
-| typed_Var x τ α :
-  (Γ x = τ) →
-  (Γ; α ⊢ₑ (Var x) : τ; α)
-| typed_App e₁ e₂ γ α β δ σ τ :
-  (Γ; γ ⊢ₑ e₁ : (Tarr σ α τ β); δ) →
-  (Γ; β ⊢ₑ e₂ : σ; γ) →
-  (Γ; α ⊢ₑ (App e₁ e₂) : τ; δ)
-| typed_AppCont e₁ e₂ α β δ σ τ :
-  (Γ; δ ⊢ₑ e₁ : (Tcont τ α); β) →
-  (Γ; σ ⊢ₑ e₂ : τ; δ) →
-  (Γ; σ ⊢ₑ (AppCont e₁ e₂) : α; β)
-| typed_NatOp o e₁ e₂ α β :
-  (Γ; α ⊢ₑ e₁ : Tnat; β) →
-  (Γ; α ⊢ₑ e₂ : Tnat; β) →
-  (Γ; α ⊢ₑ NatOp o e₁ e₂ : Tnat; β)
-| typed_If e e₁ e₂ α β σ τ :
-  (Γ; σ ⊢ₑ e : Tnat; β) →
-  (Γ; α ⊢ₑ e₁ : τ; σ) →
-  (Γ; α ⊢ₑ e₂ : τ; σ) →
-  (Γ; α ⊢ₑ (if e then e₁ else e₂) : τ; β)
-| typed_Shift (e : @expr (inc S)) τ α σ β :
-  (Γ ▹ (Tcont τ α); σ ⊢ₑ e : σ; β) →
-  (Γ; α ⊢ₑ Shift e : τ; β)
-| typed_Reset e α σ τ :
-  (Γ; σ ⊢ₑ e : σ; τ) →
-  (Γ; α ⊢ₑ reset e : τ; α)
-where "Γ ';' α '⊢ₑ' e ':' τ ';' β" := (typed_expr Γ α e τ β) : types
-with typed_val {S : Set} (Γ : S -> ty) : ty -> val S -> ty -> ty -> Prop :=
-| typed_LitV n α :
-  (Γ; α ⊢ᵥ #n : Tnat; α)
-| typed_RecV (e : expr (inc (inc S))) (δ σ τ α β : ty) :
-  ((Γ ▹ (Tarr σ α τ β) ▹ σ); α ⊢ₑ e : τ; β) ->
-  (Γ; δ ⊢ᵥ (RecV e) : (Tarr σ α τ β); δ)
-| typed_ContV (k : cont S) τ α β :
-  (Γ; α ⊢ᵪ k : τ; β) →
-  (Γ; α ⊢ᵥ (ContV k) : τ; β)
-where "Γ ';' α '⊢ᵥ' e ':' τ ';' β" := (typed_val Γ α e τ β) : types
-with typed_cont {S : Set} (Γ : S -> ty) : ty -> cont S -> ty -> ty -> Prop :=
-| typed_END τ δ :
-  (Γ; δ ⊢ᵪ END : (Tcont τ τ); δ)
-| typed_IfK e₁ e₂ α β δ A k τ :
-  (Γ; α ⊢ₑ e₁ : τ; β) ->
-  (Γ; α ⊢ₑ e₂ : τ; β) ->
-  (Γ; β ⊢ᵪ k : Tcont τ A; δ) ->
-  (Γ; α ⊢ᵪ IfK e₁ e₂ k : Tcont Tnat A; δ)
-(* | typed_AppLK v k α β σ δ τ' τ : *)
-(*   (Γ; α ⊢ᵥ v : τ'; β) -> *)
-(*   (Γ; β ⊢ᵪ k : Tcont σ τ; δ) -> *)
-(*   (Γ; α ⊢ᵪ AppLK v k : Tcont (Tarr τ' α σ δ) τ; δ) *)
-(* | typed_AppRK e k τ : *)
-(*   (Γ; τ ⊢ᵪ AppRK e k : τ; τ) *)
-(* | typed_AppContLK v k τ : *)
-(*   (Γ; τ ⊢ᵪ AppContLK v k : τ; τ) *)
-(* | typed_AppContRK e k τ : *)
-(*   (Γ; τ ⊢ᵪ AppContRK e k : τ; τ) *)
-| typed_NatOpLK op v k α β δ τ :
-  (Γ; α ⊢ᵥ v : Tnat; β) ->
-  (Γ; β ⊢ᵪ k : Tcont Tnat τ; δ) ->
-  (Γ; α ⊢ᵪ NatOpLK op v k : Tcont Tnat τ; δ)
-| typed_NatOpRK op e k α β δ τ :
-  (Γ; α ⊢ₑ e : Tnat; β) ->
-  (Γ; β ⊢ᵪ k : Tcont Tnat τ; δ) ->
-  (Γ; α ⊢ᵪ NatOpRK op e k : Tcont Tnat τ; δ)
-where "Γ ';' α '⊢ᵪ' e ':' τ ';' β" := (typed_cont Γ α e τ β) : types
-.
+(* Inductive typed_expr {S : Set} (Γ : S -> ty) : ty -> expr S -> ty -> ty -> Prop := *)
+(* | typed_Val v α τ β : *)
+(*   (Γ; α ⊢ᵥ v : τ; β) → *)
+(*   (Γ; α ⊢ₑ v : τ; β) *)
+(* | typed_Var x τ α : *)
+(*   (Γ x = τ) → *)
+(*   (Γ; α ⊢ₑ (Var x) : τ; α) *)
+(* | typed_App e₁ e₂ γ α β δ σ τ : *)
+(*   (Γ; γ ⊢ₑ e₁ : (Tarr σ α τ β); δ) → *)
+(*   (Γ; β ⊢ₑ e₂ : σ; γ) → *)
+(*   (Γ; α ⊢ₑ (App e₁ e₂) : τ; δ) *)
+(* | typed_AppCont e₁ e₂ α β δ σ τ : *)
+(*   (Γ; δ ⊢ₑ e₁ : (Tcont τ α); β) → *)
+(*   (Γ; σ ⊢ₑ e₂ : τ; δ) → *)
+(*   (Γ; σ ⊢ₑ (AppCont e₁ e₂) : α; β) *)
+(* | typed_NatOp o e₁ e₂ α β : *)
+(*   (Γ; α ⊢ₑ e₁ : Tnat; β) → *)
+(*   (Γ; α ⊢ₑ e₂ : Tnat; β) → *)
+(*   (Γ; α ⊢ₑ NatOp o e₁ e₂ : Tnat; β) *)
+(* | typed_If e e₁ e₂ α β σ τ : *)
+(*   (Γ; σ ⊢ₑ e : Tnat; β) → *)
+(*   (Γ; α ⊢ₑ e₁ : τ; σ) → *)
+(*   (Γ; α ⊢ₑ e₂ : τ; σ) → *)
+(*   (Γ; α ⊢ₑ (if e then e₁ else e₂) : τ; β) *)
+(* | typed_Shift (e : @expr (inc S)) τ α σ β : *)
+(*   (Γ ▹ (Tcont τ α); σ ⊢ₑ e : σ; β) → *)
+(*   (Γ; α ⊢ₑ Shift e : τ; β) *)
+(* | typed_Reset e α σ τ : *)
+(*   (Γ; σ ⊢ₑ e : σ; τ) → *)
+(*   (Γ; α ⊢ₑ reset e : τ; α) *)
+(* where "Γ ';' α '⊢ₑ' e ':' τ ';' β" := (typed_expr Γ α e τ β) : types *)
+(* with typed_val {S : Set} (Γ : S -> ty) : ty -> val S -> ty -> ty -> Prop := *)
+(* | typed_LitV n α : *)
+(*   (Γ; α ⊢ᵥ #n : Tnat; α) *)
+(* | typed_RecV (e : expr (inc (inc S))) (δ σ τ α β : ty) : *)
+(*   ((Γ ▹ (Tarr σ α τ β) ▹ σ); α ⊢ₑ e : τ; β) -> *)
+(*   (Γ; δ ⊢ᵥ (RecV e) : (Tarr σ α τ β); δ) *)
+(* | typed_ContV (k : cont S) τ α β : *)
+(*   (Γ; α ⊢ᵪ k : τ; β) → *)
+(*   (Γ; α ⊢ᵥ (ContV k) : τ; β) *)
+(* where "Γ ';' α '⊢ᵥ' e ':' τ ';' β" := (typed_val Γ α e τ β) : types *)
+(* with typed_cont {S : Set} (Γ : S -> ty) : ty -> cont S -> ty -> ty -> Prop := *)
+(* | typed_END τ δ : *)
+(*   (Γ; δ ⊢ᵪ END : (Tcont τ τ); δ) *)
+(* | typed_IfK e₁ e₂ α β δ A k τ : *)
+(*   (Γ; α ⊢ₑ e₁ : τ; β) -> *)
+(*   (Γ; α ⊢ₑ e₂ : τ; β) -> *)
+(*   (Γ; β ⊢ᵪ k : Tcont τ A; δ) -> *)
+(*   (Γ; α ⊢ᵪ IfK e₁ e₂ k : Tcont Tnat A; δ) *)
+(* (* | typed_AppLK v k α β σ δ τ' τ : *) *)
+(* (*   (Γ; α ⊢ᵥ v : τ'; β) -> *) *)
+(* (*   (Γ; β ⊢ᵪ k : Tcont σ τ; δ) -> *) *)
+(* (*   (Γ; α ⊢ᵪ AppLK v k : Tcont (Tarr τ' α σ δ) τ; δ) *) *)
+(* (* | typed_AppRK e k τ : *) *)
+(* (*   (Γ; τ ⊢ᵪ AppRK e k : τ; τ) *) *)
+(* (* | typed_AppContLK v k τ : *) *)
+(* (*   (Γ; τ ⊢ᵪ AppContLK v k : τ; τ) *) *)
+(* (* | typed_AppContRK e k τ : *) *)
+(* (*   (Γ; τ ⊢ᵪ AppContRK e k : τ; τ) *) *)
+(* | typed_NatOpLK op v k α β δ τ : *)
+(*   (Γ; α ⊢ᵥ v : Tnat; β) -> *)
+(*   (Γ; β ⊢ᵪ k : Tcont Tnat τ; δ) -> *)
+(*   (Γ; α ⊢ᵪ NatOpLK op v k : Tcont Tnat τ; δ) *)
+(* | typed_NatOpRK op e k α β δ τ : *)
+(*   (Γ; α ⊢ₑ e : Tnat; β) -> *)
+(*   (Γ; β ⊢ᵪ k : Tcont Tnat τ; δ) -> *)
+(*   (Γ; α ⊢ᵪ NatOpRK op e k : Tcont Tnat τ; δ) *)
+(* where "Γ ';' α '⊢ᵪ' e ':' τ ';' β" := (typed_cont Γ α e τ β) : types *)
+(* . *)
 
 Open Scope stdpp_scope.
 
@@ -113,22 +115,26 @@ Section logrel.
   Context `{!invGS Σ}.
   Context `{!stateG rs R Σ}.
   Notation iProp := (iProp Σ).
-  Notation restO := (gState_rest
-                       (@sR_idx _ _
-                          (sReifier_NotCtxDep_CtxDep reify_delim)) rs ♯ IT).
+  Notation restO
+    := (gState_rest
+          (@sR_idx _ _
+             (sReifier_NotCtxDep_CtxDep reify_delim)) rs ♯ IT).
 
   Canonical Structure exprO S := leibnizO (expr S).
   Canonical Structure valO S := leibnizO (val S).
   Canonical Structure contO S := leibnizO (cont S).
+  Canonical Structure mcontO S := leibnizO (Mcont S).
 
-  Notation "'WP' α {{ β , Φ } }" := (wp rs α notStuck ⊤ (λ β, Φ))
-                                      (at level 20, α, Φ at level 200,
-                                        format "'WP'  α  {{  β ,  Φ  } }")
+  Notation "'WP' α {{ β , Φ } }"
+    := (wp rs α notStuck ⊤ (λ β, Φ))
+         (at level 20, α, Φ at level 200,
+           format "'WP'  α  {{  β ,  Φ  } }")
       : bi_scope.
 
-  Notation "'WP' α {{ Φ } }" := (wp rs α notStuck ⊤ Φ)
-                                  (at level 20, α, Φ at level 200,
-                                    format "'WP'  α  {{  Φ  } }") : bi_scope.
+  Notation "'WP' α {{ Φ } }"
+    := (wp rs α notStuck ⊤ Φ)
+         (at level 20, α, Φ at level 200,
+           format "'WP'  α  {{  Φ  } }") : bi_scope.
 
   Definition logrel_nat' (βv : ITV) : iProp :=
     (∃ (n : natO), βv ≡ RetV n)%I.
@@ -136,228 +142,52 @@ Section logrel.
   Proof. solve_proper. Qed.
   Definition logrel_nat : ITV -n> iProp := λne x, logrel_nat' x.
 
-  (* --------- *)
-  (* Program Definition logrel_expr' *)
-  (*   (f : (ITV -n> iProp) -n> (ITV -n> iProp) -n> ITV -n> iProp) *)
-  (*   (τ α β : ITV -n> iProp) *)
-  (*   (βe : IT) : iProp := *)
-  (*   (∀ (σ : stateF ♯ IT) (κ : HOM), *)
-  (*      f τ α (FunV (Next κ)) *)
-  (*      -∗ has_substate ((laterO_map κ :: σ) : sReifier_state reify_delim ♯ IT) *)
-  (*      -∗ WP (𝒫 βe) {{ βv, β βv ∗ has_substate σ }})%I. *)
-  (* Local Instance logrel_expr_ne *)
-  (*   : (∀ n, Proper (dist n *)
-  (*                     ==> dist n *)
-  (*                     ==> dist n *)
-  (*                     ==> dist n *)
-  (*                     ==> dist n *)
-  (*                     ==> dist n) *)
-  (*             logrel_expr'). *)
-  (* Proof. solve_proper. Qed. *)
-  (* Program Definition logrel_expr *)
-  (*   : ((ITV -n> iProp) -n> (ITV -n> iProp) -n> ITV -n> iProp) *)
-  (*     -n> (ITV -n> iProp) -n> (ITV -n> iProp) -n> (ITV -n> iProp) *)
-  (*                                                 -n> IT -n> iProp := *)
-  (*   λne x y z w v, logrel_expr' x y z w v. *)
-  (* Solve All Obligations with solve_proper. *)
-
-  (* Program Definition logrel_cont_pre *)
-  (*   : ((ITV -n> iProp) -n> (ITV -n> iProp) -n> ITV -n> iProp) *)
-  (*     -n> ((ITV -n> iProp) -n> (ITV -n> iProp) -n> ITV -n> iProp) := *)
-  (*   λne μ τ α βv, *)
-  (*   (∃ (f : HOM), (IT_of_V βv) ≡ (Fun (Next f)) *)
-  (*                 ∧ □ ∀ αv, τ αv → ∀ (β : ITV -n> iProp), *)
-  (*      ▷ (logrel_expr μ α β β (`f (IT_of_V αv))))%I. *)
-  (* Solve All Obligations with solve_proper. *)
-
-  (* Local Instance logrel_cont_pre_contr : Contractive logrel_cont_pre. *)
-  (* Proof. solve_contractive. Qed. *)
-
-  (* Definition logrel_cont : (ITV -n> iProp) -n> (ITV -n> iProp) -n> ITV -n> iProp *)
-  (*   := fixpoint logrel_cont_pre. *)
-  (* Lemma logrel_cont_unfold τ α βv : *)
-  (*   logrel_cont τ α βv *)
-  (*     ≡ ((∃ (f : HOM), (IT_of_V βv) ≡ (Fun (Next (`f))) *)
-  (*                      ∧ □ ∀ αv, τ αv → ∀ (β : ITV -n> iProp), *)
-  (*           ▷ (logrel_expr logrel_cont α β β (`f (IT_of_V αv))))%I). *)
-  (* Proof. apply (fixpoint_unfold logrel_cont_pre _). Qed. *)
-
-  (* Program Definition logrel_arr' (τ α σ β : ITV -n> iProp) (βf : ITV) : iProp := *)
-  (*   (∃ f, IT_of_V βf ≡ Fun f *)
-  (*         ∧ □ ∀ (βv : ITV), *)
-  (*      τ βv -∗ logrel_expr logrel_cont σ α β (APP' (Fun f) (IT_of_V βv)))%I. *)
-  (* Local Instance logrel_arr_ne *)
-  (*   : (∀ n, Proper (dist n *)
-  (*                     ==> dist n *)
-  (*                     ==> dist n *)
-  (*                     ==> dist n *)
-  (*                     ==> dist n *)
-  (*                     ==> dist n) *)
-  (*             logrel_arr'). *)
-  (* Proof. solve_proper. Qed. *)
-  (* Program Definition logrel_arr *)
-  (*   : (ITV -n> iProp) *)
-  (*     -n> (ITV -n> iProp) *)
-  (*         -n> (ITV -n> iProp) *)
-  (*             -n> (ITV -n> iProp) -n> ITV -n> iProp := *)
-  (*   λne x y z w v, logrel_arr' x y z w v. *)
-  (* Solve All Obligations with solve_proper. *)
-
-  (* Fixpoint interp_ty (τ : ty) : ITV -n> iProp := *)
-  (*   match τ with *)
-  (*   | Tnat => logrel_nat *)
-  (*   | Tcont α β => logrel_cont (interp_ty α) (interp_ty β) *)
-  (*   | Tarr τ α σ β => logrel_arr (interp_ty τ) (interp_ty α) *)
-  (*                      (interp_ty σ) (interp_ty β) *)
-  (*   end. *)
-
-  (* Definition logrel (τ α β : ty) : IT -n> iProp *)
-  (*   := logrel_expr logrel_cont (interp_ty τ) (interp_ty α) (interp_ty β). *)
-
-  (* Local Instance interp_ty_persistent (τ : ty) α : *)
-  (*   Persistent (interp_ty τ α). *)
-  (* Proof. *)
-  (*   revert α. induction τ=> α; simpl. *)
-  (*   - unfold logrel_nat. apply _. *)
-  (*   - unfold logrel_arr. apply _. *)
-  (*   - unfold logrel_cont. *)
-  (*     rewrite logrel_cont_unfold. *)
-  (*     apply _. *)
-  (* Qed. *)
-  (* ---- *)
-
-  (* -------------------------------------- *)
-
-  Program Definition has_cont_stack : stateF ♯ IT -> iProp := λ σ,
-      (has_substate (σ : sReifier_state reify_delim ♯ IT)
-       ∗ ([∗ list] (x : laterO IT -n> laterO IT) ∈ σ,
-           ∃ (κ : HOM), x ≡ (laterO_map κ)))%I.
-
-  Lemma wp_shift (σ : stateF ♯ IT) (f : (laterO IT -n> laterO IT) -n> laterO IT)
-    (k : IT -n> IT) β {Hk : IT_hom k} Φ :
-    laterO_map 𝒫 (f (laterO_map k)) ≡ Next β →
-    has_cont_stack σ -∗
-    ▷ (£ 1 -∗ has_cont_stack σ -∗ WP β {{ Φ }}) -∗
-    WP (k (SHIFT f)) {{ Φ }}.
-  Proof.
-    iIntros (Hp) "(Hs & G) Ha".
-    iApply (wp_shift with "[Hs]"); [done | done |].
-    iNext.
-    iIntros "HCr Hs".
-    iApply ("Ha" with "HCr").
-    iFrame.
-  Qed.
-
-  Lemma wp_reset (σ : stateF ♯ IT) (e : IT) (k : IT -n> IT) {Hk : IT_hom k}
-    Φ :
-    has_cont_stack σ -∗
-    ▷ (£ 1 -∗ has_cont_stack ((laterO_map k) :: σ) -∗
-       WP 𝒫 e {{ Φ }}) -∗
-    WP k $ (RESET (Next e)) {{ Φ }}.
-  Proof.
-    iIntros "(Hs & G) Ha".
-    iApply (wp_reset with "[Hs]"); [done |].
-    iNext.
-    iIntros "HCr Hs".
-    iApply ("Ha" with "HCr").
-    iFrame.
-    unshelve eset (F := exist _ k _ : HOM); first done.
-    iExists F.
-    now subst F.
-  Qed.
-
-  Lemma wp_pop_end (v : IT)
-    {HV : AsVal v}
-    Φ :
-    has_cont_stack [] -∗
-    ▷ (£ 1 -∗ has_cont_stack [] -∗ WP v {{ Φ }}) -∗
-    WP 𝒫 v {{ Φ }}.
-  Proof.
-    iIntros "(Hs & G) Ha".
-    iApply (wp_pop_end with "Hs").
-    iNext.
-    iIntros "HCr Hs".
-    iApply ("Ha" with "HCr").
-    now iFrame.
-  Qed.
-
-  Lemma wp_pop_cons (σ : stateF ♯ IT) (v : IT) (k : IT -n> IT)
-    {HV : AsVal v}
-    Φ :
-    has_cont_stack ((laterO_map k) :: σ) -∗
-    ▷ (£ 1 -∗ has_cont_stack σ -∗ WP k $ v {{ Φ }}) -∗
-    WP 𝒫 v {{ Φ }}.
-  Proof.
-    iIntros "(Hs & (_ & G)) Ha".
-    iApply (wp_pop_cons with "Hs").
-    iNext.
-    iIntros "HCr Hs".
-    iApply ("Ha" with "HCr").
-    iFrame.
-  Qed.
-
-  Lemma wp_app_cont (σ : stateF ♯ IT) (e : laterO IT) (k' : laterO (IT -n> IT))
-    (k : IT -n> IT) β {Hk : IT_hom k}
-    Φ :
-    laterO_ap k' e ≡ Next β →
-    has_cont_stack σ -∗
-    ▷ (£ 1 -∗ has_cont_stack ((laterO_map k) :: σ) -∗
-       WP β {{ Φ }}) -∗
-    WP k (APP_CONT e k') {{ Φ }}.
-  Proof.
-    iIntros (Hb) "(Hs & G) Ha".
-    iApply (wp_app_cont with "Hs");
-      first done.
-    iNext.
-    iIntros "HCr Hs".
-    iApply ("Ha" with "HCr").
-    iFrame.
-    unshelve eset (F := exist _ k _ : HOM); first done.
-    iExists F.
-    now subst F.
-  Qed.
-
-  Definition obs_ref' (P : ITV -n> iProp) (t : IT) : iProp :=
-    (∀ (σ : stateF ♯ IT),
-       has_cont_stack σ
-       -∗ WP t {{ βv, ∃ σ',
-                        P βv ∗ has_cont_stack σ' }})%I.
-  Local Instance obs_ref_ne : NonExpansive2 obs_ref'.
+  Definition obs_ref'
+    (t : IT) (κ : HOM) (σ : stateF ♯ IT)
+    : iProp :=
+    (has_substate σ -∗ WP (𝒫 (`κ t)) {{ βv, has_substate [] }})%I.
+  Local Instance obs_ref_ne : NonExpansive3 obs_ref'.
   Proof. solve_proper. Qed.
-  Program Definition obs_ref : (ITV -n> iProp) -n> IT -n> iProp :=
-    λne x y, obs_ref' x y.
+  Program Definition obs_ref : IT -n> HOM -n> (stateF ♯ IT) -n> iProp :=
+    λne x y z, obs_ref' x y z.
   Solve All Obligations with solve_proper.
 
-  Program Definition logrel_cont'
-    (Pτ Pα : ITV -n> iProp) (k : ITV)
+  Definition logrel_mcont' (P : ITV -n> iProp) (F : stateF ♯ IT) :=
+    (∀ αv, P αv -∗ obs_ref (IT_of_V αv) HOM_id F)%I.
+  Local Instance logrel_mcont_ne : NonExpansive2 logrel_mcont'.
+  Proof. solve_proper. Qed.
+  Program Definition logrel_mcont : (ITV -n> iProp) -n> (stateF ♯ IT) -n> iProp
+    := λne x y, logrel_mcont' x y.
+  Solve All Obligations with solve_proper.
+
+  Program Definition logrel_ectx'
+    (Pτ Pα : ITV -n> iProp) (κ : HOM)
     : iProp :=
-    (∃ (f : HOM),
-       (IT_of_V k) ≡ (Fun (Next f))
-       ∧ □ ∀ αv, Pτ αv -∗ obs_ref Pα ((`f) (IT_of_V αv)))%I.
+    (□ ∀ αv, Pτ αv -∗ ∀ σ, logrel_mcont Pα σ -∗ obs_ref (IT_of_V αv) κ σ)%I.
+  Local Instance logrel_ectx_ne : NonExpansive3 logrel_ectx'.
+  Proof. solve_proper. Qed.
+  Program Definition logrel_ectx
+    : (ITV -n> iProp) -n> (ITV -n> iProp) -n> HOM -n> iProp
+    := λne x y z, logrel_ectx' x y z.
+  Solve All Obligations with solve_proper.
+
+  Program Definition logrel_cont' V W (βv : ITV) : iProp :=
+    (∃ (κ : HOM), (IT_of_V βv) ≡
+                    (Fun (Next (λne x, Tau (laterO_map (𝒫 ◎ `κ) (Next x)))))
+                  ∧ □ logrel_ectx V W κ)%I.
   Local Instance logrel_cont_ne : NonExpansive3 logrel_cont'.
   Proof. solve_proper. Qed.
   Program Definition logrel_cont
-    : (ITV -n> iProp) -n> (ITV -n> iProp) -n> ITV -n> iProp :=
-    λne x y z, logrel_cont' x y z.
+    : (ITV -n> iProp) -n> (ITV -n> iProp) -n> ITV -n> iProp
+    := λne x y z, logrel_cont' x y z.
   Solve All Obligations with solve_proper.
 
-  Program Definition logrel_expr' (Pτ Pα Pβ : ITV -n> iProp)
-    (e : IT) : iProp :=
-    (∀ (σ : stateF ♯ IT) (κ : HOM),
-       logrel_cont Pτ Pα (FunV (Next κ))
-       -∗ has_cont_stack ((laterO_map κ :: σ) : sReifier_state reify_delim ♯ IT)
-       -∗ WP (𝒫 e) {{ βv, ∃ σ', Pβ βv ∗ has_cont_stack σ' }})%I.
-  Local Instance logrel_expr_ne : NonExpansive4 logrel_expr'.
-  Proof. solve_proper. Qed.
-  Program Definition logrel_expr
-    : (ITV -n> iProp) -n> (ITV -n> iProp) -n> (ITV -n> iProp) -n> IT -n> iProp :=
-    λne x y z w, logrel_expr' x y z w.
-  Solve All Obligations with solve_proper.
-
-  Program Definition logrel_arr' (Pτ Pα Pσ Pβ : ITV -n> iProp) (f : ITV) : iProp :=
-    (∃ f', IT_of_V f ≡ Fun f'
-          ∧ □ ∀ (βv : ITV),
-       Pτ βv -∗ logrel_expr Pσ Pα Pβ (APP' (Fun f') (IT_of_V βv)))%I.
+  Program Definition logrel_arr' (Pτ Pα Pσ Pβ : ITV -n> iProp) (f : ITV) : iProp
+    := (∃ f', IT_of_V f ≡ Fun f'
+              ∧ □ ∀ (βv : ITV),
+          Pτ βv -∗ ∀ (κ : HOM),
+          logrel_ectx Pσ Pα κ -∗ ∀ σ,
+          logrel_mcont Pβ σ -∗ obs_ref (APP' (Fun f') (IT_of_V βv)) κ σ)%I.
   Local Instance logrel_arr_ne
     : (∀ n, Proper (dist n
                       ==> dist n
@@ -392,61 +222,185 @@ Section logrel.
     - unfold logrel_cont. apply _.
   Qed.
 
+  Program Definition logrel_expr (τ α δ : ITV -n> iProp) : IT -n> iProp
+    := λne e, (∀ E, logrel_ectx τ α E
+                    -∗ ∀ F, logrel_mcont δ F
+                            -∗ obs_ref e E F)%I.
+  Solve All Obligations with solve_proper.
+
   Definition logrel (τ α β : ty) : IT -n> iProp
     := logrel_expr (interp_ty τ) (interp_ty α) (interp_ty β).
 
   Program Definition ssubst_valid {S : Set}
     (Γ : S -> ty)
     (ss : interp_scope S) : iProp :=
-    (∀ x α, □ logrel (Γ x) α α (ss x))%I.
+    (∀ x τ, □ logrel (Γ x) τ τ (ss x))%I.
 
-  (* TODO: continuation *)
   Program Definition valid {S : Set}
     (Γ : S -> ty)
     (e : interp_scope S -n> IT)
-    (τ α β : ty) : iProp :=
-    (∀ γ, ssubst_valid Γ γ
-           -∗ logrel τ α β (e γ))%I.
+    (τ α σ : ty) : iProp :=
+    (□ ∀ γ, ssubst_valid Γ γ
+          -∗ logrel τ α σ (e γ))%I.
+
+  Lemma compat_empty P :
+    ⊢ logrel_mcont P [].
+  Proof.
+    iIntros (v) "Pv HH".
+    iApply (wp_pop_end with "HH").
+    iNext.
+    iIntros "_ HHH".
+    by iApply wp_val.
+  Qed.
+
+  Lemma compat_cons P Q (x : HOM) (xs : list (later IT -n> later IT)) :
+    ⊢ logrel_ectx P Q x
+      -∗ logrel_mcont Q xs
+      -∗ logrel_mcont P (laterO_map (𝒫 ◎ `x) :: xs).
+  Proof.
+    iIntros "#H G".
+    iIntros (v) "Hv Hst".
+    iApply (wp_pop_cons with "Hst").
+    iNext.
+    iIntros "_ Hst".
+    iSpecialize ("H" $! v with "Hv").
+    iApply ("H" $! xs with "G Hst").
+  Qed.
+
+  Lemma compat_HOM_id P :
+    ⊢ logrel_ectx P P HOM_id.
+  Proof.
+    iIntros (v).
+    iModIntro.
+    iIntros "Pv".
+    iIntros (σ) "Hσ HH".
+    iApply ("Hσ" with "Pv HH").
+  Qed.
+
+  Lemma logrel_of_val τ α v :
+    interp_ty α v -∗ logrel α τ τ (IT_of_V v).
+  Proof.
+    iIntros "#H".
+    iIntros (κ) "Hκ".
+    iIntros (σ) "Hσ Hown".
+    iApply ("Hκ" with "H Hσ Hown").
+  Qed.
 
   Lemma compat_var {S : Set} (Γ : S -> ty) (x : S) :
     ⊢ (∀ α, valid Γ (interp_var x) (Γ x) α α).
   Proof.
-    iIntros (α γ) "Hss".
-    iApply "Hss".
+    iIntros (α).
+    iModIntro.
+    iIntros (γ) "#Hss".
+    iIntros (E) "HE".
+    iIntros (F) "HF".
+    iIntros "Hσ".
+    iApply ("Hss" with "HE HF Hσ").
   Qed.
 
-  Lemma logrel_of_val τ α v :
-    interp_ty τ v -∗ logrel τ α α (IT_of_V v).
+  Lemma compat_reset {S : Set} (Γ : S -> ty) e σ τ :
+    ⊢ valid Γ e σ σ τ -∗ (∀ α, valid Γ (interp_reset rs e) τ α α).
   Proof.
     iIntros "#H".
-    iIntros (σ κ) "#Hκ".
-    iIntros "Hs".
-    iApply (wp_pop_cons with "Hs").
-    iDestruct "Hκ" as "(%f & #HEQ & Hκ)".
-    iPoseProof (Fun_inj' with "HEQ") as "HEQ'".
+    iIntros (α).
+    iModIntro.
+    iIntros (γ) "Hγ".
+    iIntros (κ) "Hκ".
+    iIntros (m) "Hm Hst".
+    assert (𝒫 ((`κ) (interp_reset rs e γ))
+              ≡ (𝒫 ◎ `κ) (interp_reset rs e γ)) as ->.
+    { reflexivity. }
+    iApply (wp_reset with "Hst").
     iNext.
-    iIntros "HCr Hσ".
-    unshelve eset (F := (λne βv, interp_ty α βv)%I : ITV -n> iProp);
-      first solve_proper.
-    iSpecialize ("Hκ" $! v with "H").
-    iSpecialize ("Hκ" $! σ with "Hσ").
-    subst F.
-    iAssert ((`κ) (IT_of_V v) ≡ (`f) (IT_of_V v))%I as "HEQ''".
+    iIntros "_ Hst".
+    iSpecialize ("H" $! γ with "Hγ").
+    iSpecialize ("H" $! HOM_id (compat_HOM_id _) (laterO_map (𝒫 ◎ `κ) :: m)).
+    iAssert (logrel_mcont (interp_ty τ) (laterO_map (𝒫 ◎ `κ) :: m))
+      with "[Hm Hκ]" as "Hm".
     {
-      unshelve iApply (f_equivI (λne (f : IT -n> IT),
-                           f (IT_of_V v)) (`κ) (`f) with "HEQ'"); solve_proper.
+      iIntros (v) "Hv Hst".
+      iApply (wp_pop_cons with "Hst").
+      iNext.
+      iIntros "_ Hst".
+      iSpecialize ("Hκ" $! v with "Hv").
+      iSpecialize ("Hκ" $! m with "Hm").
+      iSpecialize ("Hκ" with "Hst").
+      iApply "Hκ".
     }
-    iRewrite "HEQ''".
-    iExact "Hκ".
+    iSpecialize ("H" with "Hm Hst").
+    iApply "H".
+  Qed.
+
+  Program Definition 𝒫_HOM : @HOM sz CtxDep R _ rs := exist _ 𝒫 _.
+  Next Obligation.
+    apply _.
+  Qed.
+
+  Lemma compat_shift {S : Set} (Γ : S -> ty) e σ α τ β :
+    ⊢ valid (Γ ▹ (Tcont τ α)) e σ σ β -∗ valid Γ (interp_shift _ e) τ α β.
+  Proof.
+    iIntros "#H".
+    iModIntro.
+    iIntros (γ) "#Hγ".
+    iIntros (κ) "#Hκ".
+    iIntros (m) "Hm Hst".
+    assert (𝒫 ((`κ) (interp_shift rs e γ))
+              ≡ (𝒫 ◎ `κ) (interp_shift rs e γ)) as ->.
+    { reflexivity. }
+    iApply (wp_shift with "Hst").
+    { rewrite laterO_map_Next; reflexivity. }
+    iNext.
+    iIntros "_ Hst".
+    match goal with
+    | |- context G [ofe_mor_car _ _ e ?a] =>
+        set (γ' := a)
+    end.
+    iAssert (ssubst_valid (Γ ▹ Tcont τ α) γ') with "[Hγ Hκ]" as "Hγ'".
+    {
+      iIntros (x τ').
+      destruct x as [| x].
+      - iModIntro.
+        subst γ'.
+        iIntros (E) "HE".
+        iIntros (F) "HF Hst".
+        simpl.
+        match goal with
+        | |- context G [ofe_mor_car _ _ (`E) (ofe_mor_car _ _ Fun ?a)] =>
+            set (f := a)
+        end.
+        iApply ("HE" $! (FunV f) with "[Hκ] HF Hst").
+        iExists κ.
+        iSplit.
+        + subst f; iPureIntro.
+          reflexivity.
+        + iApply "Hκ".
+      - iApply "Hγ".
+    }
+    iSpecialize ("H" $! γ' with "Hγ'").
+    iSpecialize ("H" $! HOM_id (compat_HOM_id _) m with "Hm Hst").
+    iApply "H".
+  Qed.
+
+  Lemma compat_nat {S : Set} (Γ : S → ty) n α :
+    ⊢ valid Γ (interp_nat rs n) Tnat α α.
+  Proof.
+    iModIntro.
+    iIntros (γ) "#Hγ".
+    assert ((interp_nat rs n γ) ≡ IT_of_V (RetV n)) as ->.
+    { reflexivity. }
+    iApply logrel_of_val.
+    iExists _; by iPureIntro.
   Qed.
 
   Lemma compat_recV {S : Set} (Γ : S -> ty)
     τ1 α τ2 β e :
-    ⊢ □ valid ((Γ ▹ (Tarr τ1 α τ2 β) ▹ τ1)) e τ2 α β
+    ⊢ valid ((Γ ▹ (Tarr τ1 α τ2 β) ▹ τ1)) e τ2 α β
       -∗ (∀ θ, valid Γ (interp_rec rs e) (Tarr τ1 α τ2 β) θ θ).
   Proof.
     iIntros "#H".
-    iIntros (θ γ) "#Henv".
+    iIntros (θ).
+    iModIntro.
+    iIntros (γ) "#Hγ".
     set (f := (ir_unf rs e γ)).
     iAssert (interp_rec rs e γ ≡ IT_of_V $ FunV (Next f))%I as "Hf".
     { iPureIntro. apply interp_rec_unfold. }
@@ -458,225 +412,508 @@ Section logrel.
     iModIntro.
     iLöb as "IH".
     iIntros (v) "#Hw".
-    iIntros (σ κ) "#Hκ Hσ".
+    iIntros (κ) "#Hκ".
+    iIntros (σ) "Hσ Hst".
     rewrite APP_APP'_ITV APP_Fun laterO_map_Next -Tick_eq.
-    pose (γ' := (extend_scope (extend_scope γ (interp_rec rs e γ)) (IT_of_V v))).
+    pose (γ' :=
+            (extend_scope (extend_scope γ (interp_rec rs e γ)) (IT_of_V v))).
     rewrite /logrel.
+    Opaque extend_scope.
+    simpl.
+    rewrite hom_tick.
+    rewrite hom_tick.
+    iApply wp_tick.
+    iNext.
     iSpecialize ("H" $! γ' with "[Hw]").
     {
       iIntros (x).
       destruct x as [| [| x]]; iIntros (ξ); iModIntro.
       * iApply logrel_of_val.
         iApply "Hw".
-      * simpl.
+      * iIntros (κ') "Hκ'".
+        iIntros (σ') "Hσ' Hst".
+        Transparent extend_scope.
+        simpl.
         iRewrite "Hf".
-        iIntros (σ' κ') "Hκ' Hσ'".
-        iApply (wp_pop_cons with "Hσ'").
-        iDestruct "Hκ'" as "(%g & #HEQ & Hκ')".
-        Transparent IT_of_V.
-        iDestruct (Fun_inj' with "HEQ") as "HEQ'".
-        iNext.
-        iIntros "HCr Hσ'".
-        iSpecialize ("Hκ'" $! (FunV (Next f))).
-        iSpecialize ("Hκ'" with "[]").
+        iSpecialize ("Hκ'" $! (FunV (Next f)) with "[IH]").
         {
           iExists (Next f).
           iSplit; first done.
           iModIntro.
-          iIntros (v') "Hv'".
-          by iApply "IH".
+          iIntros (βv) "Hβv".
+          iIntros (κ'') "Hκ''".
+          iIntros (σ'') "Hσ'' Hst".
+          iApply ("IH" $! βv with "Hβv Hκ'' Hσ'' Hst").
         }
-        iSpecialize ("Hκ'" $! σ' with "Hσ'").
-        iAssert ((`κ') (IT_of_V (FunV (Next f)))
-                   ≡ (`g) (IT_of_V (FunV (Next f))))%I as "HEQ''".
-        {
-          unshelve iPoseProof
-            (f_equivI (λne (f' : IT -n> IT),
-                 f' (Fun (Next f))) (`κ') (`g) with "[HEQ']") as "GGG";
-            first solve_proper; first solve_proper; first done.
-          iApply "GGG".
-        }
-        simpl.
-        iRewrite "HEQ''".
-        iExact "Hκ'".
-      * iApply "Henv".
+        iApply ("Hκ'" $! σ' with "Hσ' Hst").
+      * iApply "Hγ".
     }
-    Opaque extend_scope.
-    simpl.
-    rewrite hom_tick.
-    iApply wp_tick.
-    iNext.
     subst γ'.
-    iApply ("H" with "Hκ Hσ").
+    iApply ("H" with "Hκ Hσ Hst").
   Qed.
 
-  Program Definition 𝒫_HOM : @HOM sz CtxDep R _ _ := exist _ 𝒫 _.
-  Next Obligation. apply _. Qed.
+  Program Definition AppContRSCtx_HOM {S : Set}
+    (α : @interp_scope F R _ S -n> IT)
+    (env : @interp_scope F R _ S)
+    : HOM := exist _ (interp_app_contrk rs α (λne env, idfun) env) _.
+  Next Obligation.
+    intros; simpl.
+    apply _.
+  Qed.
 
-  Lemma compat_reset {S : Set} (Γ : S -> ty) e σ τ :
-        ⊢ valid Γ e σ σ τ -∗ (∀ α, valid Γ (interp_reset rs e) τ α α).
+  Program Definition AppContLSCtx_HOM {S : Set}
+    (β : IT) (env : @interp_scope F R _ S)
+    (Hv : AsVal β)
+    : HOM := exist _ (interp_app_contlk rs (constO β) (λne env, idfun) env) _.
+  Next Obligation.
+    intros; simpl.
+    simple refine (IT_HOM _ _ _ _ _); intros; simpl.
+    - intros ???.
+      do 2 f_equiv.
+      intros ?; simpl.
+      solve_proper.
+    - rewrite get_val_ITV.
+      rewrite get_val_ITV.
+      simpl.
+      rewrite get_fun_tick.
+      reflexivity.
+    - rewrite get_val_ITV.
+      simpl. rewrite get_fun_vis. simpl.
+      f_equiv.
+      intros ?; simpl.
+      apply later_map_ext.
+      intros ?; simpl.
+      rewrite get_val_ITV.
+      simpl.
+      reflexivity.
+    - rewrite get_val_ITV. simpl. rewrite get_fun_err. reflexivity.
+  Qed.
+
+  Program Definition NatOpRSCtx_HOM {S : Set} (op : nat_op)
+    (α : @interp_scope F R _ S -n> IT) (env : @interp_scope F R _ S)
+    : HOM := exist _ (interp_natoprk rs op α (λne env, idfun) env) _.
+  Next Obligation.
+    intros; simpl.
+    apply _.
+  Qed.
+
+  Program Definition NatOpLSCtx_HOM {S : Set} (op : nat_op)
+    (α : IT) (env : @interp_scope F R _ S)
+    (Hv : AsVal α)
+    : HOM := exist _ (interp_natoplk rs op (constO α) (λne env, idfun) env) _.
+  Next Obligation.
+    intros; simpl.
+    apply _.
+  Qed.
+
+  Program Definition AppRSCtx_HOM {S : Set}
+    (α : @interp_scope F R _ S -n> IT)
+    (env : @interp_scope F R _ S)
+    : HOM := exist _ (interp_apprk rs α (λne env, idfun) env) _.
+  Next Obligation.
+    intros; simpl.
+    apply _.
+  Qed.
+
+  Program Definition AppLSCtx_HOM {S : Set}
+    (β : IT) (env : @interp_scope F R _ S)
+    (Hv : AsVal β)
+    : HOM := exist _ (interp_applk rs (constO β) (λne env, idfun) env) _.
+  Next Obligation.
+    intros; simpl.
+    apply _.
+  Qed.
+
+  Lemma compat_nat_op {S : Set} (Γ : S → ty)
+    D E F e1 e2 op :
+    ⊢ valid Γ e1 Tnat E F
+      -∗ valid Γ e2 Tnat F D
+      -∗ valid Γ (interp_natop rs op e1 e2) Tnat E D.
   Proof.
-    iIntros "H".
-    iIntros (α γ) "#Henv".
-    iIntros (σ' κ) "#Hκ Hσ'".
-    iApply (wp_reset with "Hσ'").
-    iNext.
-    iIntros "HCr Hσ'".
-    iSpecialize ("H" $! γ with "Henv").
-    iSpecialize ("H" $! (laterO_map (`κ) :: σ') 𝒫_HOM with "[] Hσ'").
-    {
-      iExists 𝒫_HOM.
-      iSplit; first done.
-      iModIntro.
-      iIntros (v) "#Hv".
-      iIntros (σ'') "Hσ''".
-      destruct σ'' as [| κ' σ''].
-      - simpl.
-        iApply (wp_pop_end with "Hσ''").
-        iNext.
-        iIntros "HC Hs".
-        iApply wp_val.
-        iModIntro.
-        iExists [].
-        iFrame "Hs Hv".
-      - simpl.
-        simpl in κ'.
-        iDestruct "Hσ''" as "(H1 & #H2)".
-        rewrite big_opL_cons.
-        iDestruct "H2" as "((%κκ & Hκκ) & H2)".
-        iRewrite "Hκκ" in "H1".
-        iApply (delim.wp_pop_cons with "H1").
-        iNext.
-        iIntros "HC Hs".
-        iDestruct "Hκ" as "(%g & #HEQ & #Hκ)".
-        iSpecialize ("Hκ" $! v).
-        (* pop cons different rule with extra tick *)
-        admit.
-    }
-    (* push continuation forward *)
-    iApply (wp_wand with "H").
-    iIntros (v) "(%s & #G1 & G2)".
+    iIntros "#H #G".
     iModIntro.
-    iExists s.
-    iFrame.
-    admit.
-  Admitted.
+    iIntros (γ) "#Hγ".
+    iIntros (κ) "#Hκ".
+    iIntros (m) "Hm Hst".
+    rewrite /interp_natop //=.
 
-  Lemma compat_shift {S : Set} (Γ : S -> ty) e σ α τ β :
-    ⊢ valid (Γ ▹ (Tcont τ α)) e σ σ β -∗ valid Γ (interp_shift _ e) τ α β.
-  Proof.
-    iIntros "H".
-    iIntros (γ) "#Henv".
-    iIntros (σ' κ) "#Hκ Hσ'".
-    iApply (wp_shift with "Hσ'").
-    { apply (laterO_map_Next 𝒫). }
+    set (κ' := (NatOpRSCtx_HOM op e1 γ)).
+    assert ((NATOP (do_natop op) (e1 γ) (e2 γ)) = ((`κ') (e2 γ))) as -> by done.
+    rewrite HOM_ccompose.
+    pose (sss := (HOM_compose κ κ')). rewrite (HOM_compose_ccompose κ κ' sss)//.
+
+    iSpecialize ("G" $! γ with "Hγ").
+    iSpecialize ("G" $! sss).
+    iApply ("G" with "[H] Hm Hst").
+
+    iIntros (w).
+    iModIntro.
+    iIntros "#Hw".
+    iIntros (m') "Hm Hst".
+    subst sss.
+    subst κ'.
+    simpl.
+
+    pose (κ' := (NatOpLSCtx_HOM op (IT_of_V w) γ _)).
+    assert ((NATOP (do_natop op) (e1 γ) (IT_of_V w)) = ((`κ') (e1 γ)))
+      as -> by done.
+    rewrite HOM_ccompose.
+    pose (sss := (HOM_compose κ κ')). rewrite (HOM_compose_ccompose κ κ' sss)//.
+
+    iSpecialize ("H" $! γ with "Hγ").
+    iSpecialize ("H" $! sss).
+    iApply ("H" with "[] Hm Hst").
+
+    iIntros (v).
+    iModIntro.
+    iIntros "#Hv".
+    iIntros (m'') "Hm Hst".
+    subst sss.
+    subst κ'.
+    simpl.
+
+    iDestruct "Hw" as "(%n & #HEQ1)".
+    iDestruct "Hv" as "(%n' & #HEQ2)".
+    iSpecialize ("Hκ" $! (RetV (do_natop op n' n)) with "[]").
     {
-      iNext.
-      iIntros "HCr Hσ'".
-      set (F := (FunV (Next (λne x : IT, Tau (laterO_map 𝒫 (Next x))))) : ITV).
-      iSpecialize ("H" $! (extend_scope γ (IT_of_V F)) with "[Hκ]").
-      - iIntros (x τ').
-        iDestruct "Hκ" as "(%g & #HEQ & #Hκ)".
-        iIntros (σ'' κ').
-        iModIntro.
-        iIntros "Hκ' Hσ''".
-        destruct x as [| x].
-        + Transparent extend_scope.
-          iApply (wp_pop_cons with "Hσ''").
-          iDestruct (Fun_inj' with "HEQ") as "HEQ''".
-          iDestruct "Hκ'" as "(%h & #HEQ' & #Hκ')".
-          iDestruct (Fun_inj' with "HEQ'") as "HEQ'''".
-          iSpecialize ("Hκ'" $! F).
-          iNext.
-          iIntros "HCr Hs".
-          iApply (wp_wand with "[Hκ' Hs]").
-          {
-            iAssert ((`κ') (extend_scope γ (IT_of_V F) VZ)
-                       ≡ (`h) (extend_scope γ (IT_of_V F) VZ))%I as "HEQ''''".
-            {
-              unshelve iPoseProof (f_equivI (λne (f' : IT -n> IT), f' (extend_scope γ (IT_of_V F) VZ)) (`κ') (`h) with "[HEQ']") as "GGG";
-                first solve_proper; first solve_proper;
-                first done.
-              iApply "GGG".
-            }
-            iRewrite "HEQ''''".
-            iApply "Hκ'"; last iApply "Hs".
-            simpl.
-            unfold logrel_cont'.
-            subst F.
-            unshelve eset (F' := exist _ (λne x : IT, Tau (laterO_map 𝒫 (Next x))) _ : HOM).
-            {
-              simpl.
-              econstructor.
-              - intros.
-                rewrite ->2 later_map_Next.
-                rewrite hom_tick.
-                rewrite <- Tick_eq.
-                rewrite <- Tick_eq.
-                reflexivity.
-              - intros.
-                rewrite -> later_map_Next.
-                rewrite hom_vis.
-                rewrite <- Tick_eq.
-                admit.
-              - intros.
-                rewrite -> later_map_Next.
-                rewrite hom_err.
-                admit.
-            }
-            iExists F'.
-            iSplit; first done.
-            iModIntro.
-            iIntros (v) "HHH".
-            subst F'.
-            simpl.
-            rewrite later_map_Next.
-            iIntros (s) "Hs".
-            rewrite <- Tick_eq.
-            iApply wp_tick.
-            iNext.
-            destruct s as [| x s].
-            - iApply (wp_pop_end with "Hs").
-              iNext.
-              iIntros "HCr Hs".
-              iApply wp_val.
-              iModIntro.
-              iExists [].
-              iFrame "Hs".
-              admit.
-            - admit.
-          }
-          iIntros (v) "HHH".
-          iModIntro.
-          iApply "HHH".
-        + iApply ("Henv" with "[Hκ'] Hσ''").
-          iApply "Hκ'".
-      - subst F.
-        Opaque extend_scope.
-        simpl.
-        unfold logrel_expr'.
-        simpl.
-        iSpecialize ("H" $! σ' κ).
-
-        admit.
+      iExists _.
+      iPureIntro.
+      reflexivity.
     }
-  Admitted.
+    iSpecialize ("Hκ" $! m'' with "Hm Hst").
+    rewrite IT_of_V_Ret.
+
+    iAssert ((NATOP (do_natop op) (IT_of_V v) (IT_of_V w))
+               ≡ (Ret (do_natop op n' n)))%I as "#HEQ".
+    {
+      iRewrite "HEQ1".
+      rewrite IT_of_V_Ret.
+      iAssert ((IT_of_V v) ≡ IT_of_V (RetV n'))%I as "#HEQ2'".
+      {
+        iApply f_equivI.
+        iApply "HEQ2".
+      }
+      rewrite IT_of_V_Ret.
+      iAssert (NATOP (do_natop op) (IT_of_V v) (Ret n)
+                 ≡ NATOP (do_natop op) (Ret n') (Ret n))%I as "#HEQ2''".
+      {
+        unshelve iApply (f_equivI (λne x, NATOP (do_natop op) x (Ret n))).
+        { solve_proper. }
+        { solve_proper. }
+        iApply "HEQ2'".
+      }
+      iRewrite "HEQ2''".
+      rewrite NATOP_Ret.
+      done.
+    }
+    iRewrite "HEQ".
+    iApply "Hκ".
+  Qed.
+
+  Lemma compat_app {S : Set} (Γ : S → ty)
+    A B C D E F e1 e2 :
+    ⊢ valid Γ e1 (Tarr A C B E) E F
+      -∗ valid Γ e2 A F D
+      -∗ valid Γ (interp_app rs e1 e2) B C D.
+  Proof.
+    iIntros "#H #G".
+    iModIntro.
+    iIntros (γ) "#Hγ".
+    iIntros (κ) "#Hκ".
+    iIntros (σ) "Hσ Hst".
+    rewrite /interp_app //=.
+
+    pose (κ' := (AppRSCtx_HOM e1 γ)).
+    assert ((e1 γ ⊙ (e2 γ)) = ((`κ') (e2 γ))) as ->.
+    { simpl; unfold AppRSCtx. reflexivity. }
+    assert ((`κ) ((`κ') (e2 γ)) = ((`κ) ◎ (`κ')) (e2 γ)) as ->.
+    { reflexivity. }
+    pose (sss := (HOM_compose κ κ')).
+    assert ((`κ ◎ `κ') = (`sss)) as ->.
+    { reflexivity. }
+
+    iSpecialize ("G" $! γ with "Hγ").
+    iSpecialize ("G" $! sss).
+    iApply ("G" with "[H] Hσ Hst").
+
+    iIntros (w).
+    iModIntro.
+    iIntros "#Hw".
+    iIntros (m') "Hm Hst".
+    subst sss.
+    subst κ'.
+    simpl.
+
+    pose (κ'' := (AppLSCtx_HOM (IT_of_V w) γ _)).
+    assert (((`κ) (e1 γ ⊙ (IT_of_V w))) = (((`κ) ◎ (`κ'')) (e1 γ))) as ->.
+    { reflexivity. }
+    pose (sss := (HOM_compose κ κ'')).
+    assert ((`κ ◎ `κ'') = (`sss)) as ->.
+    { reflexivity. }
+
+    iSpecialize ("H" $! γ with "Hγ").
+    iSpecialize ("H" $! sss).
+    iApply ("H" with "[] Hm Hst").
+
+    iIntros (v).
+    iModIntro.
+    iIntros "#Hv".
+    iIntros (m'') "Hm Hst".
+    subst sss.
+    subst κ''.
+    simpl.
+
+    iDestruct "Hv" as "(%n' & #HEQ & Hv)".
+    iSpecialize ("Hv" $! w with "Hw").
+    iSpecialize ("Hv" $! κ with "Hκ").
+    iSpecialize ("Hv" $! m'' with "Hm Hst").
+    iAssert ((IT_of_V v ⊙ (IT_of_V w))
+               ≡ (Fun n' ⊙ (IT_of_V w)))%I as "#HEQ'".
+    {
+      iApply (f_equivI (λne x, (x ⊙ (IT_of_V w)))).
+      iApply "HEQ".
+    }
+    iRewrite "HEQ'".
+    iApply "Hv".
+  Qed.
 
   Lemma compat_appcont {S : Set} (Γ : S -> ty) e1 e2 τ α δ β σ :
-    valid Γ e1 (Tcont τ α) δ β
-    -∗ valid Γ e2 τ σ δ
+    valid Γ e1 (Tcont τ α) σ δ
+    -∗ valid Γ e2 τ δ β
     -∗ valid Γ (interp_app_cont _ e1 e2) α σ β.
   Proof.
-    iIntros "H G".
+    iIntros "#H #G".
+    iModIntro.
     iIntros (γ) "#Henv".
-    iIntros (σ' κ) "#Hκ Hσ'".
-    iSpecialize ("H" $! γ with "Henv").
+    iIntros (κ) "#Hκ".
+    iIntros (σ') "Hm Hst".
+
+    pose (κ' := (AppContRSCtx_HOM e1 γ)).
+    assert ((interp_app_cont rs e1 e2 γ) = ((`κ') (e2 γ))) as ->.
+    { simpl. reflexivity. }
+    assert ((`κ) ((`κ') (e2 γ)) = ((`κ) ◎ (`κ')) (e2 γ)) as ->.
+    { reflexivity. }
+    pose (sss := (HOM_compose κ κ')).
+    assert ((`κ ◎ `κ') = (`sss)) as ->.
+    { reflexivity. }
+
     iSpecialize ("G" $! γ with "Henv").
-    iSpecialize ("H" $! σ').
-    iSpecialize ("G" $! σ').
-    (* (* bind + pop *) *)
-    admit.
+    iSpecialize ("G" $! sss).
+    iApply ("G" with "[H] Hm Hst").
+
+    iIntros (w).
+    iModIntro.
+    iIntros "#Hw".
+    iIntros (m') "Hm Hst".
+    subst sss.
+    subst κ'.
+    Opaque interp_app_cont.
+    simpl.
+
+    pose (κ'' := (AppContLSCtx_HOM (IT_of_V w) γ _)).
+    set (F := (`κ) _).
+    assert (F ≡ (((`κ) ◎ (`κ'')) (e1 γ))) as ->.
+    {
+      subst F. simpl. Transparent interp_app_cont. simpl.
+      f_equiv.
+      rewrite ->2 get_val_ITV.
+      simpl.
+      reflexivity.
+    }
+    pose (sss := (HOM_compose κ κ'')).
+    assert ((`κ ◎ `κ'') = (`sss)) as ->.
+    { reflexivity. }
+
+    iSpecialize ("H" $! γ with "Henv").
+    iSpecialize ("H" $! sss).
+    iApply ("H" with "[] Hm Hst").
+
+    iIntros (v).
+    iModIntro.
+    iIntros "#Hv".
+    iIntros (m'') "Hm Hst".
+    subst sss.
+    subst κ''.
+    Opaque APP_CONT.
+    simpl.
+
+    rewrite get_val_ITV.
+    simpl.
+
+    iDestruct "Hv" as "(%n' & #HEQ & #Hv)".
+    iRewrite "HEQ".
+    rewrite get_fun_fun.
+    simpl.
+
+    match goal with
+    | |- context G [ofe_mor_car _ _
+                     (ofe_mor_car _ _ APP_CONT ?a) ?b] =>
+        set (T := APP_CONT a b)
+    end.
+    iAssert (𝒫 ((`κ) T) ≡ (𝒫 ◎ (`κ)) T)%I as "HEQ'".
+    { iPureIntro. reflexivity. }
+    iRewrite "HEQ'"; iClear "HEQ'".
+    subst T.
+
+    iApply (wp_app_cont with "[Hst]").
+    { reflexivity. }
+    - iFrame "Hst".
+    - simpl.
+      iNext.
+      iIntros "_ Hst".
+      rewrite later_map_Next.
+      rewrite <-Tick_eq.
+      iApply wp_tick.
+      iNext.
+      iSpecialize ("Hv" $! w with "Hw").
+
+      iApply ("Hv" $! (laterO_map (𝒫 ◎ `κ) :: m'') with "[Hm] Hst").
+      {
+        iIntros (p) "#Hp Hst".
+        iApply (wp_pop_cons with "Hst").
+        iNext.
+        iIntros "_ Hst".
+        iApply ("Hκ" with "Hp Hm Hst").
+      }
+
+  Qed.
+
+  Program Definition valid_ectx {S : Set}
+    (Γ : S -> ty)
+    (e : interp_scope S -n> IT -n> IT)
+    `{∀ γ, IT_hom (e γ)}
+    (τ α : ty) : iProp :=
+    (□ ∀ γ, ssubst_valid Γ γ
+            -∗ logrel_ectx (interp_ty τ) (interp_ty α) (exist _ (e γ) _))%I.
+  Next Obligation.
+    intros; apply _.
+  Qed.
+
+  (* bla-bla done *)
+  Lemma compat_natop_r {S : Set} (Γ : S → ty) α τ
+    op t (E : interp_scope S -n> IT -n> IT)
+    `{∀ γ, IT_hom (E γ)}
+    `{∀ γ, IT_hom (interp_natoprk _ op t E γ)} :
+    ⊢ valid_ectx Γ E Tnat τ
+      -∗ valid Γ t Tnat τ α
+      -∗ valid_ectx Γ (interp_natoprk _ op t E) Tnat α.
+  Proof.
+    iIntros "#H #G".
+    iIntros (γ).
+    iModIntro.
+    iIntros "#Hγ".
+    iIntros (v).
+    iModIntro.
+    iIntros "#Hv".
+    iIntros (m) "Hm Hst".
+
+    pose (κ' := (NatOpLSCtx_HOM op (IT_of_V v) γ _)).
+    simpl.
+    assert (E γ (NATOP (do_natop op) (t γ) (IT_of_V v)) = ((E γ ◎ `κ') (t γ)))
+      as -> by done.
+    iSpecialize ("G" $! γ with "Hγ").
+    unshelve iApply ("G" $! (exist _ (E γ ◎ `κ') _) with "[] Hm Hst").
+    { apply _. }
+    simpl.
+
+    iIntros (w).
+    iModIntro.
+    iIntros "#Hw".
+    iIntros (m') "Hm Hst".
+    simpl.
+
+    iSpecialize ("H" $! γ with "Hγ").
   Admitted.
+
+  (* bla-bla done *)
+  Lemma compat_natop_l {S : Set} (Γ : S → ty) α τ
+    op (t : interp_scope S -n> IT) (E : interp_scope S -n> IT -n> IT)
+    `{∀ γ, IT_hom (E γ)}
+    `{∀ γ, AsVal (t γ)}
+    `{∀ γ, IT_hom (interp_natoplk _ op t E γ)} :
+    ⊢ valid_ectx Γ E Tnat τ
+      -∗ valid Γ t Tnat τ α
+      -∗ valid_ectx Γ (interp_natoplk _ op t E) Tnat α.
+  Proof.
+    iIntros "#H #G".
+    iIntros (γ).
+    iModIntro.
+    iIntros "#Hγ".
+    iIntros (v).
+    iModIntro.
+    iIntros "#Hv".
+    iIntros (m) "Hm Hst".
+    simpl.
+    pose (κ' := (NATOP (do_natop op) (IT_of_V v))).
+    simpl.
+    assert (E γ (NATOP (do_natop op) (IT_of_V v) (t γ)) = ((E γ ◎ κ') (t γ)))
+      as -> by done.
+    iSpecialize ("G" $! γ with "Hγ").
+    unshelve iApply ("G" $! (exist _ (E γ ◎ κ') _) with "[] Hm Hst").
+    { apply _. }
+    subst κ'.
+    simpl.
+
+    iIntros (w).
+    iModIntro.
+    iIntros "#Hw".
+    iIntros (m') "Hm Hst".
+    simpl.
+
+    iSpecialize ("H" $! γ with "Hγ").
+  Admitted.
+
+  (* Lemma compat_app_l {S : Set} (Γ : S → ty) τ α c d e *)
+  (*   (* (t : interp_scope S -n> ITVO) *) t *)
+  (*   (E : interp_scope S -n> IT -n> IT) *)
+  (*   `{∀ γ, IT_hom (E γ)} *)
+  (*   (* `{∀ γ, AsVal (t γ)} *) *)
+  (*   `{∀ γ, IT_hom (interp_app_contlk _ t E γ)} : *)
+  (*   ⊢ valid_ectx Γ E τ α *)
+  (*     -∗ valid Γ t c d e *)
+  (*     -∗ valid_ectx Γ (interp_app_contlk _ t E) τ α. *)
+  (* Proof.     *)
+  (*   iIntros "#H #G". *)
+  (*   iIntros (γ). *)
+  (*   assert (AsVal (t γ)); first admit. *)
+  (*   iModIntro. *)
+  (*   iIntros "#Hγ". *)
+  (*   iIntros (v). *)
+  (*   iModIntro. *)
+  (*   iIntros "#Hv". *)
+  (*   iIntros (m) "Hm Hst". *)
+  (*   simpl. *)
+  (*   rewrite get_val_ITV. *)
+  (*   simpl. *)
+  (*   iSpecialize ("H" $! γ with "Hγ"). *)
+  (*   iSpecialize ("H" $! v with "Hv"). *)
+  (*   iSpecialize ("H" $! m with "Hm Hst"). *)
+  (*   simpl. *)
+
+  (* Lemma compat_app_r {S : Set} (Γ : S → ty) τ α c d e t *)
+  (*   (E : interp_scope S -n> IT -n> IT) *)
+  (*   `{∀ γ, IT_hom (E γ)} *)
+  (*   `{∀ γ, IT_hom (interp_app_contrk _ t E γ)} : *)
+  (*   ⊢ valid_ectx Γ E τ α *)
+  (*     -∗ valid Γ t c d e *)
+  (*     -∗ valid_ectx Γ (interp_app_contrk _ t E) τ α.   *)
+  (* Proof. *)
+  (*   iIntros "#H #G". *)
+  (*   iIntros (γ). *)
+  (*   iModIntro. *)
+  (*   iIntros "#Hγ". *)
+  (*   iIntros (v). *)
+  (*   iModIntro. *)
+  (*   iIntros "#Hv". *)
+  (*   iIntros (m) "Hm Hst". *)
+  (*   simpl. *)
+  (*   rewrite get_val_ITV. *)
+  (*   simpl. *)
+  (*   iSpecialize ("H" $! γ with "Hγ"). *)
+  (*   iSpecialize ("H" $! v with "Hv"). *)
+  (*   iSpecialize ("H" $! m with "Hm Hst"). *)
+  (*   simpl. *)
+  (* Qed. *)
 
 End logrel.
 
@@ -685,36 +922,40 @@ Local Definition rs : gReifiers CtxDep 1 := gReifiers_cons reify_delim gReifiers
 Variable Hdisj : ∀ (Σ : gFunctors) (P Q : iProp Σ), disjunction_property P Q.
 
 Lemma logpred_adequacy cr Σ R `{!Cofe R, SubOfe natO R}
-  `{!invGpreS Σ} `{!statePreG rs R Σ} τ β'
+  `{!invGpreS Σ} `{!statePreG rs R Σ} τ
   (α : interp_scope ∅ -n> IT (gReifiers_ops rs) R)
-  (β : IT (gReifiers_ops rs) R) st st' k :
+  (e : IT (gReifiers_ops rs) R) st' k :
   (∀ `{H1 : !invGS Σ} `{H2: !stateG rs R Σ},
-      (£ cr ⊢ valid rs □ α τ τ β')%I) →
-  ssteps (gReifiers_sReifier rs) (𝒫 (α ı_scope)) st β st' k →
-  (∃ β1 st1, sstep (gReifiers_sReifier rs) β st' β1 st1)
-   ∨ (∃ βv, IT_of_V βv ≡ β).
+      (£ cr ⊢ valid rs □ α τ τ τ)%I) →
+  ssteps (gReifiers_sReifier rs) (𝒫 (α ı_scope)) ([], ()) e st' k →
+  (∃ β1 st1, sstep (gReifiers_sReifier rs) e st' β1 st1)
+   ∨ (∃ βv, IT_of_V βv ≡ e).
 Proof.
   intros Hlog Hst.
-  destruct (IT_to_V β) as [βv|] eqn:Hb.
+  destruct (IT_to_V e) as [βv|] eqn:Hb.
   { right. exists βv. apply IT_of_to_V'. rewrite Hb; eauto. }
   left.
-  cut ((∃ β1 st1, sstep (gReifiers_sReifier rs) β st' β1 st1)
-      ∨ (∃ e, β ≡ Err e ∧ notStuck e)).
+  cut ((∃ β1 st1, sstep (gReifiers_sReifier rs) e st' β1 st1)
+      ∨ (∃ e', e ≡ Err e' ∧ notStuck e')).
   { intros [?|He]; first done.
     destruct He as [? [? []]]. }
   eapply (wp_safety cr); eauto.
   { apply Hdisj. }
   { by rewrite Hb. }
   intros H1 H2.
-  exists (λ _, True)%I. split. (* (interp_ty _ τ)%I *)
+  exists (λ _, True)%I. split.
   { apply _. }
   iIntros "[Hcr  Hst]".
   iPoseProof (Hlog with "Hcr") as "Hlog".
-  destruct st as [σ []].
-  iAssert (has_substate σ) with "[Hst]" as "Hs".
+  match goal with
+  | |- context G [has_full_state (?a, _)] =>
+      set (st := a)
+  end.
+  simpl in st.
+  iAssert (has_substate _) with "[Hst]" as "Hs".
   { unfold has_substate, has_full_state.
-    assert (of_state rs (IT (gReifiers_ops rs) _) (σ,()) ≡
-            of_idx rs (IT (gReifiers_ops rs) _) sR_idx (sR_state σ)) as ->; last done.
+    eassert (of_state rs (IT (gReifiers_ops rs) _) (_,()) ≡
+            of_idx rs (IT (gReifiers_ops rs) _) sR_idx (sR_state _)) as ->; last done.
     intro j. unfold sR_idx. simpl.
     unfold of_state, of_idx.
     destruct decide as [Heq|]; last first.
@@ -723,28 +964,26 @@ Proof.
     inv_fin j; last done.
     intros Heq.
     rewrite (eq_pi _ _ Heq eq_refl)//.
+    simpl.
+    unfold iso_ofe_refl.
+    cbn.
+    reflexivity.
   }
   iSpecialize ("Hlog" $! ı_scope with "[]").
   { iIntros ([]). }
-  iSpecialize ("Hlog" $! σ HOM_id with "[]").
+  iSpecialize ("Hlog" $! HOM_id (compat_HOM_id _ _) [] with "[]").
   {
-    iExists HOM_id.
-    iSplit; first done.
-    iModIntro.
-    iIntros (αv) "HHH".
-    iIntros (βv) "Hκ".
-    simpl.
+    iIntros (αv) "HHH GGG".
+    iApply (wp_pop_end with "GGG").
+    iNext.
+    iIntros "_ GGG".
     iApply wp_val.
-    iModIntro.
-    iExists βv.
-    iFrame.
+    by iModIntro.
   }
-  iSpecialize ("Hlog" with "[Hs]").
-  {
-    admit.
-  }
+  subst st.
+  iSpecialize ("Hlog" with "Hs").
   iApply (wp_wand with "Hlog").
   iIntros (βv). simpl.
   iIntros "_".
   done.
-Admitted.
+Qed.
